\documentclass{article}
\usepackage{amsmath}

\begin{document}
    Naj bo \(U(x,y) = U_{x,y}\) matrika
    \begin{align*}
        \Delta u(x,y) = U_{xx} + U_{yy}\\
        h\cdot U_x = U(x) - U(x+1)\\
        h^2\cdot U_{xx} = U(x-1, y) - 2U(x,y) + U(x+1,y)\\
        h^2\cdot U_{yy} = U(x, y-1) - 2U(x,y) + U(x, y+1)
    \end{align*}
    ÄŒe to damo skupaj, dobimo
    \begin{align*}
        \Delta U(x,y) + k(x,y)U(x,y) = 1
        h^2 = U(x-1,y)+U(x+1,y)+U(x,y-1)+U(x,y+1) + (h^2\cdot k- 4) U(x,y)
    \end{align*}
    Tako lahko sestavimo matriko \(T\)
    \begin{align*}
        T = \begin{bmatrix}
        \end{bmatrix}
    \end{align*}

\end{document}